feat: export Lean to HTML (#537)
This PR adds two executables:

* verso-literate: this uses elaborated Verso moduledocs and docstrings to create a richer representation of a Lean module than the prior literate module support, and with less overhead from heuristic Markdown processing.

* verso-html: this takes the results of verso-literate and produces an HTML rendering of source code. Perhaps ironically, this fails on Verso documents due to differences in the parser's output, but it can render the rest of Verso's source without issue.

It also adds the ability for the blog genre and the manual genre to include text using verso-literate, so they can load arbitrary Lean files with Verso moduledocs and treat them as content.

src/multi-verso/MultiVerso/Slug.lean
@@ -7,10 +7,13 @@ module
 import Std.Data.HashSet
 import Verso.Method
 public import Lean.Data.Json.FromToJson.Basic
+import Std.Tactic.BVDecide
+meta import Lean.Elab.Command
 
 public section
 
 set_option linter.missingDocs true
+set_option doc.verso true
 
 namespace Verso.Multi
 open Verso.Method
@@ -18,6 +21,55 @@ open Lean (ToJson FromJson)
 open Std (HashSet)
 
 private def validCharString := "abcdefghijklmnopqrstuvwxyzABCDEFGHIJKLMNOPQRSTUVWXYZ0123456789-_"
+
+open Lean Elab Command in
+run_cmd do
+  let x := Lean.mkIdent `x
+  let mut e ← `(False)
+  for c in validCharString.toList do
+    e ← `($x = $(Lean.quote c) ∨ $e)
+  elabCommand <| ← `(def $(mkIdent `Slug.ValidChar) ($x : Char) : Prop := $e)
+  for c in validCharString.toList do
+    elabCommand <| ← `(@[simp, grind .] theorem $(mkIdent <| `Slug.ValidChar ++ .str .anonymous s!"{c}") : $(mkIdent `Slug.ValidChar) $(quote c) := by unfold $(mkIdent `Slug.ValidChar); simp)
+
+/--
+Checks whether a character is valid in slugs (that is, whether it's an English letter, a digit, a
+dash, or an underscore).
+-/
+def Slug.validChar (c : Char) : Bool :=
+  lower c || upper c || digit c || c == '-' || c == '_'
+where
+  lower
+    | 'a' | 'b' | 'c' | 'd' | 'e' | 'f' | 'g' | 'h' | 'i' | 'j' | 'k' | 'l' | 'm' | 'n' | 'o' | 'p' | 'q' | 'r' | 's' | 't' | 'u' | 'v' | 'w' | 'x' | 'y' | 'z' => true
+    | _ => false
+  upper
+    | 'A' | 'B' | 'C' | 'D' | 'E' | 'F' | 'G' | 'H' | 'I' | 'J' | 'K' | 'L' | 'M' | 'N' | 'O' | 'P' | 'Q' | 'R' | 'S' | 'T' | 'U' | 'V' | 'W' | 'X' | 'Y' | 'Z' => true
+    | _ => false
+  digit
+    | '0' | '1' | '2' | '3' | '4' | '5' | '6' | '7' | '8' | '9' => true
+    | _ => false
+
+
+theorem Slug.validChar_eq_ValidChar {c : Char} : Slug.validChar c = Slug.ValidChar c := by
+  simp only [eq_iff_iff]
+  constructor
+  . simp [validChar]
+    intro
+    repeat' (rename_i h; cases h)
+    . rename_i h; simp [validChar.lower] at h; split at h <;> simp_all [ValidChar]
+    . rename_i h; simp [validChar.upper] at h; split at h <;> simp_all [ValidChar]
+    . rename_i h; simp [validChar.digit] at h; split at h <;> simp_all [ValidChar]
+    all_goals (simp_all [ValidChar])
+  . intro
+    repeat (rename_i h; cases h; subst_eqs; rfl)
+    contradiction
+
+instance : DecidablePred Slug.ValidChar := fun c =>
+  if h : Slug.validChar c then
+    isTrue <| by simp_all [Slug.validChar_eq_ValidChar]
+  else
+    isFalse <| by simp_all [Slug.validChar_eq_ValidChar]
+
 
 /-- The characters allowed in slugs. -/
 def Slug.validChars :=
@@ -108,23 +160,26 @@ instance : DecidableRel (@LE.le Slug _) := fun s1 s2 =>
 defmethod String.sluggify (str : String) : Slug :=
   ⟨asSlug str⟩
 
+instance : Append Slug where
+  append := private fun | ⟨s1⟩, ⟨s2⟩ => ⟨s1 ++ s2⟩
+
 /--
 Converts a string to a slug.
 -/
 def ofString (str : String) : Slug := str.sluggify
 
 /--
-Returns a slug that's not present in `used`, starting with `slug` and appending consecutive numbers
+Returns a slug that's not present in {name}`used`, starting with {name}`slug` and appending consecutive numbers
 until it becomes unique.
 
-The consecutive numbers start at `startCount`, which is `1` by default. Callers with reason to
+The consecutive numbers start at {name}`startCount`, which is {lean (type:="Nat")}`1` by default. Callers with reason to
 believe that there will be many collisions may provide an alternative starting value.
 -/
 partial def unique (used : HashSet Slug) (slug : Slug) (startCount : Nat := 1) : Slug :=
   if !(used.contains slug) then slug
   else
     let rec attempt (i : Nat) :=
-      let slug' := s!"{slug.toString}{i}".sluggify
+      let slug' := s!"{slug.toString}-{i}".sluggify
       if !(used.contains slug') then slug'
       else attempt (i + 1)
     attempt startCount
