src/tests/Tests/HtmlEntities.lean
@@ -1,0 +1,36 @@
+/-
+Copyright (c) 2025 Lean FRO LLC. All rights reserved.
+Released under Apache 2.0 license as described in the file LICENSE.
+Author: David Thrane Christiansen
+-/
+import Verso.Output.Html.Entities
+
+open Verso.Output.Html
+
+/-- info: some "&" -/
+#guard_msgs in
+#eval decodeEntity? "&amp;"
+
+/-- info: some "&" -/
+#guard_msgs in
+#eval decodeEntity? "&AMP"
+
+/-- info: some #["&AMP", "&AMP;", "&amp", "&amp;"] -/
+#guard_msgs in
+#eval namedEntity? '&' |>.map (·.toArray |>.qsort)
+
+/-- info: some " " -/
+#guard_msgs in
+#eval decodeEntity? "&#32;"
+
+/-- info: some " " -/
+#guard_msgs in
+#eval decodeEntity? "&#x20;"
+
+/-- info: none -/
+#guard_msgs in
+#eval decodeEntity? "&#;"
+
+/-- info: none -/
+#guard_msgs in
+#eval decodeEntity? "&blah;"
