src/tests/Tests/Paths.lean
@@ -1,0 +1,96 @@
+/-
+Copyright (c) 2025 Lean FRO LLC. All rights reserved.
+Released under Apache 2.0 license as described in the file LICENSE.
+Author: David Thrane Christiansen
+-/
+
+module
+
+
+import MultiVerso.Path
+
+set_option doc.verso true
+
+namespace Verso.Multi
+open Path
+
+/-! Tests for the module MultiVerso.Path -/
+
+-- TODO: adapt to module system. Right now, non-meta imports work in server, but not command line.
+/-
+/-- info: "/" -/
+#guard_msgs in
+#eval link #[]
+
+/-- info: "/a/b/" -/
+#guard_msgs in
+#eval link #["a", "b"]
+
+/-- info: "/a/b/#c" -/
+#guard_msgs in
+#eval link #["a", "b"] (htmlId := some "c")
+/- Tests for relativization. -/
+
+/-- info: "a/b/c/" -/
+#guard_msgs in
+#eval Path.relativize #[] "/a/b/c/"
+/-- info: "a/b/c/#foo" -/
+#guard_msgs in
+#eval Path.relativize #[] "/a/b/c/#foo"
+/-- info: "a/b/c#foo" -/
+#guard_msgs in
+#eval Path.relativize #[] "/a/b/c#foo"
+
+/-- info: "b/c/" -/
+#guard_msgs in
+#eval Path.relativize #["a"] "/a/b/c/"
+/-- info: "b/c/#foo" -/
+#guard_msgs in
+#eval Path.relativize #["a"] "/a/b/c/#foo"
+/-- info: "b/c#foo" -/
+#guard_msgs in
+#eval Path.relativize #["a"] "/a/b/c#foo"
+
+/-- info: "c/" -/
+#guard_msgs in
+#eval Path.relativize #["a", "b"] "/a/b/c/"
+/-- info: "c/#foo" -/
+#guard_msgs in
+#eval Path.relativize #["a", "b"] "/a/b/c/#foo"
+/-- info: "c#foo" -/
+#guard_msgs in
+#eval Path.relativize #["a", "b"] "/a/b/c#foo"
+
+/-- info: "../../aa/b/c#foo" -/
+#guard_msgs in
+#eval Path.relativize #["a", "b"] "/aa/b/c#foo"
+
+/-- info: "../" -/
+#guard_msgs in
+#eval Path.relativize #["a", "b", "c", "d"] "/a/b/c/"
+/-- info: "../../c" -/
+#guard_msgs in
+#eval Path.relativize #["a", "b", "c", "d"] "/a/b/c"
+
+/-- info: "../#foo" -/
+#guard_msgs in
+#eval Path.relativize #["a", "b", "c", "d"] "/a/b/c/#foo"
+/-- info: "../../" -/
+#guard_msgs in
+#eval Path.relativize #["a", "b", "c", "d", "e"] "/a/b/c/"
+/-- info: "../../#foo" -/
+#guard_msgs in
+#eval Path.relativize #["a", "b", "c", "d", "e"] "/a/b/c/#foo"
+/-- info: "../../../c#foo" -/
+#guard_msgs in
+#eval Path.relativize #["a", "b", "c", "d", "e"] "/a/b/c#foo"
+
+/-- info: "../../../c" -/
+#guard_msgs in
+#eval Path.relativize #["a", "b", "c", "d", "e"] "/a/b/c"
+
+/-- info: "" -/
+#guard_msgs in
+#eval Path.relativize #[] "/"
+
+-/
