src/verso-blog/VersoBlog.lean
@@ -9,6 +9,7 @@ import SubVerso.Examples
 
 import VersoBlog.Basic
 import VersoBlog.LiterateLeanPage
+import VersoBlog.LiterateModuleDocs
 import VersoBlog.Generate
 import VersoBlog.Site
 import VersoBlog.Site.Syntax
