src/verso-literate/VersoLiterate.lean
@@ -3,7 +3,8 @@ Copyright (c) 2025 Lean FRO LLC. All rights reserved.
 Released under Apache 2.0 license as described in the file LICENSE.
 Author: David Thrane Christiansen
 -/
-import Tests.Golden
-import Tests.ParserRegression
-import Tests.Paths
-import Tests.HtmlEntities
+
+import VersoLiterate.Basic
+import VersoLiterate.Exported
+import VersoLiterate.Module
+import VersoLiterate.Search
