src/verso-literate/VersoLiterate/Basic.lean
@@ -1,0 +1,409 @@
+/-
+Copyright (c) 2025 Lean FRO LLC. All rights reserved.
+Released under Apache 2.0 license as described in the file LICENSE.
+Author: David Thrane Christiansen
+-/
+
+import Lean.Elab.Term
+import Verso
+import MultiVerso
+import SubVerso.Highlighting
+import Std.Data.HashSet
+import Std.Data.TreeSet
+import Verso.BEq
+
+open Verso Doc
+open SubVerso.Highlighting
+open Lean Elab Term
+open Std
+
+namespace VersoLiterate
+
+local instance : Repr Json where
+  reprPrec v _ := "json%" ++ v.render
+
+inductive Ext where
+  | highlighted : Highlighted → Ext
+  | data : Json → Ext
+deriving ToJson, FromJson, Repr
+
+open Verso.BEq in
+instance : BEq Ext where
+  beq := ptrEqThen fun
+    | .highlighted hl1, .highlighted hl2 =>
+      ptrEqThen' hl1 hl2 (· == ·)
+    | .data x, .data y =>
+      ptrEqThen' x y (· == ·)
+    | _, _ => false
+
+def InlineToLiterate := Name → Dynamic → Array (Doc.Inline Ext) → TermElabM (Option (Doc.Inline Ext))
+def BlockToLiterate := Name → Dynamic → Array (Doc.Block Ext Ext) → TermElabM (Option (Doc.Block Ext Ext))
+
+initialize inlineToLiterateAttr : TagAttribute ← registerTagAttribute `inline_to_literate ""
+initialize blockToLiterateAttr : TagAttribute ← registerTagAttribute `block_to_literate ""
+
+namespace Builtin
+def handleLocal : InlineToLiterate
+  | ``Lean.Doc.Data.Local, val, content => do
+    if let some { name, type, lctx, fvarId } := val.get? Lean.Doc.Data.Local then
+      let (t, _) ← (Lean.Meta.ppExpr type).run {lctx := lctx} {}
+      let s := match content with | #[.code s] => s | _ => name.toString
+      let i := .other (.highlighted <| .token ⟨.var fvarId (toString t), s⟩) #[.code s]
+      return some i
+    throwError "Wrong data"
+  | _, _, _ => pure none
+
+def handleConst : InlineToLiterate
+  | ``Lean.Doc.Data.Const, val, content => do
+    if let some { name } := val.get? Lean.Doc.Data.Const then
+      let signature ← PrettyPrinter.ppSignature name
+      let docs ← findDocString? (← getEnv) name
+      let k := .const name (toString signature.fmt) docs false
+      let s := match content with | #[.code s] => s | _ => name.toString
+      let i := .other (.highlighted <| .token ⟨k, s⟩) #[.code s]
+      return some i
+    throwError "Wrong data"
+  | _, _, _ => pure none
+
+def handlePostponed : InlineToLiterate
+  | ``Lean.Doc.PostponedCheck, val, content => do
+    if let some { .. } := val.get? Lean.Doc.PostponedCheck then
+      -- TODO postponed checks need a solution here
+      return some <| .concat content
+    throwError "Wrong data"
+  | _, _, _ => pure none
+
+def highlightDocCode : Lean.Doc.DocCode → Highlighted
+  | ⟨code⟩ => Id.run do
+    let mut out : Highlighted := .empty
+    for (str, info?) in code do
+      if let some info := info? then
+        let k :=
+          match info with
+          | .const x sig
+          | .field x sig => .const x (sig.pretty 45) none false
+          | .var _ fv ty => .var fv (ty.pretty 45)
+          | .option name declName => .option name declName none
+          | .literal _litKind (some type) => .withType (type.pretty 45)
+          | .literal .. => .unknown
+          | .keyword => .keyword none none none
+        out := out ++ .token ⟨k, str⟩
+      else out := out ++ .text str
+    return out
+
+def handleTerm : InlineToLiterate
+  | ``Lean.Doc.Data.LeanTerm, val, content => do
+    if let some { term, ..} := val.get? Lean.Doc.Data.LeanTerm then
+      return some <| .other (.highlighted <| highlightDocCode term) content
+    throwError "Wrong data"
+  | _, _, _ => pure none
+
+def handleOption : InlineToLiterate
+  | ``Lean.Doc.Data.Option, val, content => do
+    if let some { name, declName } := val.get? Lean.Doc.Data.Option then
+      let str := if let #[.code s] := content then s else toString name
+      return some <| .other (.highlighted <| .token ⟨.option name declName none, str⟩) content
+    throwError "Wrong data"
+  | _, _, _ => pure none
+
+def handleModName : InlineToLiterate
+  | ``Lean.Doc.Data.ModuleName, val, content => do
+    if let some { module } := val.get? Lean.Doc.Data.ModuleName then
+      return some <| .other (.highlighted <| .token ⟨.moduleName module, module.toString⟩) content
+    throwError "Wrong data"
+  | _, _, _ => pure none
+
+def handleTactic : InlineToLiterate
+  | ``Lean.Doc.Data.Tactic, val, content => do
+    if let some { name } := val.get? Lean.Doc.Data.Tactic then
+      let s := if let #[.code s] := content then s else name.toString
+      return some <| .other (.highlighted <| .token ⟨.keyword (some name) none none, s⟩) content
+    throwError "Wrong data"
+  | _, _, _ => pure none
+
+def inline := #[handleLocal, handleConst, handlePostponed, handleTerm, handleOption, handleModName, handleTactic]
+
+end Builtin
+
+unsafe def getInlineToLiterateUnsafe [Monad m] [MonadEnv m] [MonadError m] [MonadOptions m] : m (Array InlineToLiterate) := do
+  let env ← getEnv
+  let mut all := #[]
+  for modIdx in [0:env.header.modules.size] do
+    all := all ++ inlineToLiterateAttr.ext.getModuleEntries env modIdx
+  all := all ++ (inlineToLiterateAttr.ext.getState env).toArray
+  return (← all.mapM (evalConstCheck InlineToLiterate ``InlineToLiterate)) ++ Builtin.inline
+
+@[implemented_by getInlineToLiterateUnsafe]
+opaque getInlineToLiterate [Monad m] [MonadEnv m] [MonadError m] [MonadOptions m] : m (Array InlineToLiterate)
+
+unsafe def getBlockToLiterateUnsafe [Monad m] [MonadEnv m] [MonadError m] [MonadOptions m] : m (Array BlockToLiterate) := do
+  let env ← getEnv
+  let mut all := #[]
+  for modIdx in [0:env.header.modules.size] do
+    all := all ++ inlineToLiterateAttr.ext.getModuleEntries env modIdx
+  all := all ++ (inlineToLiterateAttr.ext.getState env).toArray
+  all.mapM (evalConstCheck BlockToLiterate ``BlockToLiterate)
+
+@[implemented_by getBlockToLiterateUnsafe]
+opaque getBlockToLiterate [Monad m] [MonadEnv m] [MonadError m] [MonadOptions m] : m (Array BlockToLiterate)
+
+open Verso.Multi
+
+open Std in
+structure State where
+  htmlIds : HashMap InternalId Slug := {}
+  usedInternalIds : TreeSet InternalId := {}
+  usedHtmlIds : HashSet Slug := {}
+  /--
+  For each module, saves the HTML IDs assigned to the module docstrings. The module doc in module
+  `M`, item `i`, code element `j`, would be under keys `` `M `` and then `(i, j)`.
+  -/
+  modDocs : NameMap (HashMap (Nat × Nat) Slug) := {}
+  moduleDomain : Domain := { title := "Modules" }
+  constantDefDomain : Domain := { title := "Global constants" }
+
+section
+open Verso.BEq
+variable [BEq α] [Hashable α] [Ord α]
+
+@[inline]
+private def hashMapEq [BEq β] : (x1 x2 : HashMap α β) → Bool := ptrEqThen fun l r =>
+    l.size = r.size && l.fold (init := true) (· && r[·]?.isEqSome ·)
+
+@[inline]
+private def hashMapEqWith (eq : β → β → Bool) : (x1 x2 : HashMap α β) → Bool := ptrEqThen fun l r =>
+    l.size = r.size && l.fold (init := true) fun soFar k v => soFar && (r[k]?.map (ptrEqThen eq v)).getD false
+
+@[inline]
+private def hashSetEq : (x1 x2 : HashSet α) → Bool := ptrEqThen fun l r =>
+  l.size = r.size && l.all (· ∈ r)
+
+@[inline]
+private def treeSetEq : (x1 x2 : TreeSet α) → Bool := ptrEqThen fun l r =>
+  l.size = r.size && l.all (· ∈ r)
+
+@[inline]
+private def treeMapEqWith (eq : β → β → Bool) : (x1 x2 : TreeMap α β) → Bool := ptrEqThen fun l r =>
+  l.size = r.size && l.foldl (init := true) fun soFar k v => soFar && (r[k]?.map (ptrEqThen eq v)).getD false
+
+@[inline]
+private def nameMapEqWith (eq : β → β → Bool) : (x1 x2 : NameMap β) → Bool := ptrEqThen fun l r =>
+  l.size = r.size && l.foldl (init := true) fun soFar k v => soFar && ((r.find? k).map (ptrEqThen eq v)).getD false
+
+
+instance : BEq State where
+  beq := ptrEqThen fun
+    | ⟨u1, v1, w1, x1, y1, z1⟩, ⟨u2, v2, w2, x2, y2, z2⟩ =>
+      hashMapEq u1 u2 &&
+      treeSetEq v1 v2 &&
+      hashSetEq w1 w2 &&
+      nameMapEqWith (hashMapEqWith (· == ·)) x1 x2 &&
+      y1 == y2 &&
+      z1 == z2
+
+end
+
+def State.getDef (name : Name) (state : State) : Option Slug := do
+  let obj ← state.constantDefDomain.get? (toString name)
+  for i in obj.ids do
+    if let some x := state.htmlIds[i]? then return x
+  failure
+
+def State.definitionIds (state : State) : NameMap String :=
+  state.constantDefDomain.objects.foldl (init := {}) fun defIds name obj =>
+    if let some htmlId := obj.ids.toArray.findSome? (state.htmlIds[·]?) |>.map (·.toString) then
+      defIds.insert name.toName htmlId
+    else defIds
+
+def State.moduleLink (state : State) (mod : Name) : Option Link := do
+  if let some obj := state.moduleDomain[toString mod]? then
+    for i in obj.ids do
+      if let some htmlId := state.htmlIds[i]? then
+        return { path := mod.components.map (·.toString) |>.toArray, htmlId }
+  none
+
+def State.constLink (state : State) (c : Name) : Option Link := do
+  if let some obj := state.constantDefDomain[toString c]? then
+    if let .ok v := obj.data.getObjValAs? String "module" then
+      if let some link := state.moduleLink v.toName then
+        if let some htmlId := obj.ids.toArray.findSome? state.htmlIds.get? then
+          return { link with htmlId }
+  none
+
+def State.modDocLink (state : State) (mod : Name) (item : Nat) (pos : Nat) : Option Link := do
+  let link ← state.moduleLink mod
+  let docIds ← state.modDocs.find? mod
+  let htmlId ← docIds[(item, pos)]?
+  return { link with htmlId }
+
+def State.saveModDoc (state : State) (mod : Name) (item pos : Nat) : Slug × State :=
+  if let some x := (state.modDocs.find? mod).bind (·[(item, pos)]?) then
+    (x, state)
+  else
+    let slug := Slug.unique state.usedHtmlIds s!"mod-doc-{mod}-{item}-{pos}".sluggify
+    { fst := slug,
+      snd := { state with
+        usedHtmlIds := state.usedHtmlIds.insert slug
+        modDocs := state.modDocs.alter mod (·.getD {} |>.insert (item, pos) slug)
+      }
+    }
+
+def State.moduleIds (state : State) : NameMap String :=
+  state.moduleDomain.objects.foldl (init := {}) fun modIds name obj =>
+    if let some htmlId := obj.ids.toArray.findSome? (state.htmlIds[·]?) |>.map (·.toString) then
+      modIds.insert name.toName htmlId
+    else modIds
+
+open Verso.Multi in
+def State.allLinks (state : State) : HashMap InternalId Link := Id.run do
+  let mut idLinks := HashMap.emptyWithCapacity state.usedInternalIds.size
+  for (name, obj) in state.moduleDomain.objects do
+    if let some link := state.moduleLink name.toName then
+      for id in obj.ids do
+        idLinks := idLinks.insert id link
+  for (_, obj) in state.constantDefDomain.objects do
+      if let .ok v := obj.data.getObjValAs? String "module" then
+        if let some link := state.moduleLink v.toName then
+          if let some htmlId := obj.ids.toArray.findSome? state.htmlIds.get? then
+            for id in obj.ids do
+              idLinks := idLinks.insert id { link with htmlId }
+  return idLinks
+
+
+def State.linkTargets (state : State) : Code.LinkTargets ρ where
+  const x _ := Id.run do
+    if let some obj := state.constantDefDomain.get? x.toString then
+      if let .ok v := obj.data.getObjValAs? String "module" then
+        if let some link := state.moduleLink v.toName then
+          return #[.mk "def" s!"Definition of `{x}`" link.link]
+    return #[]
+  moduleName m _ :=
+    if let some link := state.moduleLink m then
+      #[.mk "mod" s!"Module `{m}`" link.link]
+    else #[]
+
+structure Context where
+  currentModule : Name := .anonymous
+
+def Literate : Genre where
+  PartMetadata := Empty
+  Block := Ext
+  Inline := Ext
+  TraverseContext := Context
+  TraverseState := State
+
+instance : ToJson Literate.Block := inferInstanceAs <| ToJson Ext
+instance : ToJson Literate.Inline := inferInstanceAs <| ToJson Ext
+
+instance : TraverseBlock Literate where
+instance : TraversePart Literate where
+
+abbrev TraverseM := ReaderT Context (StateRefT State IO)
+
+def freshId : TraverseM InternalId := do
+  modifyGet fun s =>
+    let (i, s') := InternalId.fresh s.usedInternalIds
+    (i, { s with usedInternalIds := s' })
+
+def freshHtmlId (name : Name) : TraverseM Slug := do
+  let mut slug := (toString name).sluggify
+  while (← get).usedHtmlIds.contains slug do
+    slug := slug ++ next
+  modify (fun st => {st with usedHtmlIds := st.usedHtmlIds.insert slug })
+  return slug
+where
+  next := "-".sluggify
+
+def saveDef (name : Name) : TraverseM Slug := do
+  let mod := (← read).currentModule
+  let data := json%{ "module": $(mod), "private": $(isPrivateName name), "userName": $(privateToUserName name) }
+  let name' := toString name
+  if let some obj := (← get).constantDefDomain.get? name' then
+    modify (fun st => { st with constantDefDomain := st.constantDefDomain.setData name' data })
+    for i in obj.ids do
+      if let some x := (← get).htmlIds[i]? then return x
+    -- No HTML ID is registered. Because all these internal IDs are aliases,
+    -- we should stick the slug on all of them and return it.
+    let x ← freshHtmlId name
+    modify (fun st => { st with htmlIds := st.htmlIds.insertMany (obj.ids.toArray.map (·, x)) })
+    return x
+  else
+    let i ← freshId
+    let x ← freshHtmlId name
+    modify fun st =>
+      { st with
+        constantDefDomain := st.constantDefDomain.insertId name' i |>.setData name' data
+        htmlIds := st.htmlIds.insert i x
+      }
+    return x
+
+def saveModule (name : Name) : TraverseM Slug := do
+  if let some obj := (← get).moduleDomain.get? (toString name) then
+    for i in obj.ids do
+      if let some x := (← get).htmlIds[i]? then return x
+    -- No HTML ID is registered. Because all these internal IDs are aliases,
+    -- we should stick the slug on all of them and return it.
+    let x ← freshHtmlId name
+    modify (fun st => { st with htmlIds := st.htmlIds.insertMany (obj.ids.toArray.map (·, x)) })
+    return x
+  else
+    let i ← freshId
+    let x ← freshHtmlId name
+    modify fun st =>
+      { st with
+        moduleDomain := st.moduleDomain.insertId (toString name) i
+        htmlIds := st.htmlIds.insert i x
+      }
+    return x
+
+def saveModDoc (mod : Name) (item pos : Nat) : TraverseM Slug := do
+  modifyGet (·.saveModDoc mod item pos)
+
+def getDef (name : Name) : TraverseM (Option Slug) := do
+  if let some obj := (← get).constantDefDomain.get? (toString name) then
+    for i in obj.ids do
+      if let some x := (← get).htmlIds[i]? then return some x
+    return none
+  else return none
+
+instance : Traverse Literate TraverseM where
+  part _ := pure none
+  block _ := pure ()
+  inline _ := pure ()
+  genrePart := nofun
+  genreBlock _ _ := pure none
+  genreInline _ _ := pure none
+
+open Html
+instance [Monad m] : GenreHtml Literate m where
+  part _ := nofun
+  block _goI goB ext contents :=
+    match ext with
+    | .highlighted hl => hl.blockHtml (g := Literate) "lean"
+    | .data _ => contents.mapM goB
+  inline goI ext contents :=
+    match ext with
+    | .highlighted hl => hl.inlineHtml (g := Literate) "lean"
+    | .data _ => contents.mapM goI
+
+
+/--
+Genres with {name}`LoadLiterate` instances allow Lean modules with module docstrings to be translated into
+documents.
+-/
+class LoadLiterate (g : Genre) where
+  inline
+    (go : Inline Literate → Inline g)
+    (container : Literate.Inline) (contents : Array (Inline Literate)) : Inline g
+  block
+    (goI : Inline Literate → Inline g) (goB : Block Literate → Block g)
+    (container : Literate.Block) (contents : Array (Block Literate)) : Block g
+
+  docstring (indent : Nat) (declName? : Option Name) (content : Array (Block g)) : Block g
+
+  docstringPart (lvl : Nat)
+    (title : Array (Inline g))
+    (content : Array (Block g)) : Block g
+
+partial def LoadLiterate.part [LoadLiterate g] (lvl : Nat) (p : Part g) : Block g :=
+  docstringPart lvl p.title (p.content ++ p.subParts.map (part (lvl + 1)))
