src/verso-literate/VersoLiterate/Search.lean
@@ -1,0 +1,16 @@
+/-
+Copyright (c) 2025 Lean FRO LLC. All rights reserved.
+Released under Apache 2.0 license as described in the file LICENSE.
+Author: David Thrane Christiansen
+-/
+
+import VersoLiterate.Basic
+import VersoSearch
+
+namespace VersoLiterate
+open Verso Search
+
+instance : Indexable Literate where
+  partId := nofun
+  block _ := none
+  inline _ := none
