src/verso-util/VersoUtil.lean
@@ -3,5 +3,5 @@ Copyright (c) 2025 Lean FRO LLC. All rights reserved.
 Released under Apache 2.0 license as described in the file LICENSE.
 Author: David Thrane Christiansen
 -/
-
-import VersoUtil.BinFiles
+module
+public import VersoUtil.BinFiles
