src/verso/Verso/Doc.lean
@@ -3,10 +3,13 @@ Copyright (c) 2023-2024 Lean FRO LLC. All rights reserved.
 Released under Apache 2.0 license as described in the file LICENSE.
 Author: David Thrane Christiansen
 -/
-
-import Lean.Data.Json
-import Lean.DocString.Types
+module
+public import Lean.Data.Json
+public import Lean.DocString.Types
 import Verso.Doc.Name
+
+set_option doc.verso true
+set_option pp.rawOnError true
 
 namespace Verso
 
@@ -20,12 +23,14 @@ open Lean.Json (getObj?)
 A genre is a kind of document that can be written with Verso.
 
 A genre is primarily defined by its extensions to the Verso framework, provided in this type.
-Additionally, each genre should provide a `main` function that is responsible for the traversal pass
+Additionally, each genre should provide a {lit}`main` function that is responsible for the traversal pass
 and for generating output.
 -/
-structure Genre : Type 1 where
+public structure Genre : Type 1 where
   /--
-  The metadata that may be associated with each `Part` (e.g. author, publication date,
+  {open Verso.Doc}
+
+  The metadata that may be associated with each {name scope:="Verso.Doc"}`Part` (e.g. author, publication date,
   cross-referencing identifier).
   -/
   PartMetadata : Type
@@ -38,8 +43,10 @@ structure Genre : Type 1 where
   -/
   Inline : Type
   /--
-  The reader-style data used in the genre's traversal pass. Instances of `TraversePart` and
-  `TraverseBlock` for a genre specify how this is updated while traversing parts and blocks,
+  {open Verso.Doc}
+
+  The reader-style data used in the genre's traversal pass. Instances of {name scope:="Verso.Doc"}`TraversePart` and
+  {name scope:="Verso.Doc"}`TraverseBlock` for a genre specify how this is updated while traversing parts and blocks,
   respectively.
   -/
   TraverseContext : Type
@@ -48,7 +55,8 @@ structure Genre : Type 1 where
   -/
   TraverseState : Type
 
-def Genre.none : Genre := ⟨Empty, Empty, Empty, Unit, Unit⟩
+@[expose]
+public def Genre.none : Genre := ⟨Empty, Empty, Empty, Unit, Unit⟩
 
 instance : Repr Genre.none.Block where
   reprPrec e _ := nomatch e
@@ -61,7 +69,7 @@ instance : Repr Genre.none.PartMetadata where
 
 export Lean.Doc (MathMode MathMode.inline MathMode.display)
 
-deriving instance ToJson, FromJson for MathMode
+deriving instance ToJson, FromJson for Lean.Doc.MathMode
 
 private def arrayEq (eq : α → α → Bool) (xs ys : Array α) : Bool := Id.run do
     if h : xs.size = ys.size then
@@ -75,55 +83,81 @@ private def arrayEq (eq : α → α → Bool) (xs ys : Array α) : Bool := Id.ru
     else return false
 
 @[inherit_doc Lean.Doc.Inline]
-abbrev Inline (genre : Genre) :=
+public abbrev Inline (genre : Genre) :=
   Lean.Doc.Inline genre.Inline
 
-@[inherit_doc Lean.Doc.Inline.text, match_pattern]
-def Inline.text (string : String) : Inline genre :=
+@[inherit_doc Lean.Doc.Inline.text, expose, match_pattern]
+public def Inline.text (string : String) : Inline genre :=
   Lean.Doc.Inline.text (string : String)
 
-@[inherit_doc Lean.Doc.Inline.emph, match_pattern]
-def Inline.emph (content : Array (Inline genre)) : Inline genre :=
+@[inherit_doc Lean.Doc.Inline.emph, expose, match_pattern]
+public def Inline.emph (content : Array (Inline genre)) : Inline genre :=
   Lean.Doc.Inline.emph (content : Array (Inline genre))
 
-@[inherit_doc Lean.Doc.Inline.bold, match_pattern]
-def Inline.bold (content : Array (Inline genre)) : Inline genre :=
+@[inherit_doc Lean.Doc.Inline.bold, expose, match_pattern]
+public def Inline.bold (content : Array (Inline genre)) : Inline genre :=
   Lean.Doc.Inline.bold (content : Array (Inline genre))
 
-@[inherit_doc Lean.Doc.Inline.code, match_pattern]
-def Inline.code (string : String) : Inline genre :=
+@[inherit_doc Lean.Doc.Inline.code, expose, match_pattern]
+public def Inline.code (string : String) : Inline genre :=
   Lean.Doc.Inline.code (string : String)
 
-@[inherit_doc Lean.Doc.Inline.math, match_pattern]
-def Inline.math (mode : MathMode) (string : String) : Inline genre :=
+@[inherit_doc Lean.Doc.Inline.math, expose, match_pattern]
+public def Inline.math (mode : MathMode) (string : String) : Inline genre :=
   Lean.Doc.Inline.math (mode : MathMode) (string : String)
 
-@[inherit_doc Lean.Doc.Inline.linebreak, match_pattern]
-def Inline.linebreak (string : String) : Inline genre :=
+@[inherit_doc Lean.Doc.Inline.linebreak, expose, match_pattern]
+public def Inline.linebreak (string : String) : Inline genre :=
   Lean.Doc.Inline.linebreak (string : String)
 
-@[inherit_doc Lean.Doc.Inline.link, match_pattern]
-def Inline.link (content : Array (Inline genre)) (url : String) : Inline genre :=
+@[inherit_doc Lean.Doc.Inline.link, expose, match_pattern]
+public def Inline.link (content : Array (Inline genre)) (url : String) : Inline genre :=
   Lean.Doc.Inline.link (content : Array (Inline genre)) (url : String)
 
-@[inherit_doc Lean.Doc.Inline.footnote, match_pattern]
-def Inline.footnote (name : String) (content : Array (Inline genre)) : Inline genre :=
+@[inherit_doc Lean.Doc.Inline.footnote, expose, match_pattern]
+public def Inline.footnote (name : String) (content : Array (Inline genre)) : Inline genre :=
   Lean.Doc.Inline.footnote (name : String) (content : Array (Inline genre))
 
-@[inherit_doc Lean.Doc.Inline.image, match_pattern]
-def Inline.image (alt : String) (url : String) : Inline genre :=
+@[inherit_doc Lean.Doc.Inline.image, expose, match_pattern]
+public def Inline.image (alt : String) (url : String) : Inline genre :=
   Lean.Doc.Inline.image (alt : String) (url : String)
 
-@[inherit_doc Lean.Doc.Inline.concat, match_pattern]
-def Inline.concat (content : Array (Inline genre)) : Inline genre :=
+@[inherit_doc Lean.Doc.Inline.concat, expose, match_pattern]
+public def Inline.concat (content : Array (Inline genre)) : Inline genre :=
   Lean.Doc.Inline.concat (content : Array (Inline genre))
 
-@[inherit_doc Lean.Doc.Inline.other, match_pattern]
-def Inline.other (container : genre.Inline) (content : Array (Inline genre)) : Inline genre :=
+@[inherit_doc Lean.Doc.Inline.other, expose, match_pattern]
+public def Inline.other (container : genre.Inline) (content : Array (Inline genre)) : Inline genre :=
   Lean.Doc.Inline.other (container : genre.Inline) (content : Array (Inline genre))
 
+public def Inline.empty : Inline genre := .concat #[]
 
-def Inline.empty : Inline genre := .concat #[]
+public partial def Inline.rewriteOtherM [Monad m]
+    (onInline :
+      (Inline genre1 → m (Inline genre2)) →
+      genre1.Inline → Array (Inline genre1) →
+      m (Inline genre2)) :
+    Inline genre1 → m (Inline genre2)
+  | .text str => pure <| .text str
+  | .linebreak str => pure <| .linebreak str
+  | .image alt url => pure <| .image alt url
+  | .code s => pure <| .code s
+  | .math m s => pure <| .math m s
+  | .emph content => .emph <$> content.mapM (rewriteOtherM onInline)
+  | .bold content => .bold <$> content.mapM (rewriteOtherM onInline)
+  | .concat content => .concat <$> content.mapM (rewriteOtherM onInline)
+  | .footnote name content => .footnote name <$> content.mapM (rewriteOtherM onInline)
+  | .link content url => (.link · url) <$> content.mapM (rewriteOtherM onInline)
+  | .other container content =>
+    onInline (rewriteOtherM onInline) container content
+
+public partial def Inline.rewriteOther
+    (onInline :
+      (Inline genre1 → Inline genre2) →
+      genre1.Inline → Array (Inline genre1) →
+      Inline genre2) :
+    Inline genre1 → Inline genre2 :=
+  Inline.rewriteOtherM (m := Id) onInline
 
 private partial def Inline.toJson [ToJson i] : Lean.Doc.Inline i → Json
   | .text str => json% {"text": $str}
@@ -138,10 +172,10 @@ private partial def Inline.toJson [ToJson i] : Lean.Doc.Inline i → Json
   | .concat content => json% {"concat": $(content.map toJson)}
   | .other container content => json%{"other": {"container": $container, "content": $(content.map toJson)}}
 
-instance instToJsonLeanInline [ToJson i] : ToJson (Lean.Doc.Inline i) where
-  toJson := Inline.toJson
+public instance instToJsonLeanInline [ToJson i] : ToJson (Lean.Doc.Inline i) where
+  toJson := private Inline.toJson
 
-@[instance] abbrev instToJsonInline [ToJson genre.Inline] : ToJson (Inline genre) := instToJsonLeanInline
+@[instance] public abbrev instToJsonInline [ToJson genre.Inline] : ToJson (Inline genre) := instToJsonLeanInline
 
 private partial def Inline.fromJson? [inst : FromJson i] (json : Json) : Except String (Lean.Doc.Inline i) := do
   let obj ← json.getObj?
@@ -175,12 +209,12 @@ private partial def Inline.fromJson? [inst : FromJson i] (json : Json) : Except 
   else
     throw "Expected a one-field object"
 
-instance instFromJsonLeanInline [FromJson i] : FromJson (Lean.Doc.Inline i) where
-  fromJson? := Inline.fromJson?
+public instance instFromJsonLeanInline [FromJson i] : FromJson (Lean.Doc.Inline i) where
+  fromJson? := private Inline.fromJson?
 
 @[instance] abbrev instFromJsonInline [FromJson genre.Inline] : FromJson (Inline genre) := instFromJsonLeanInline
 
-partial def Inline.beq [BEq i] : Lean.Doc.Inline i → Lean.Doc.Inline i → Bool
+private partial def Inline.beq [BEq i] : Lean.Doc.Inline i → Lean.Doc.Inline i → Bool
   | .text str1, .text str2
   | .code str1, .code str2
   | .linebreak str1, .linebreak str2=> str1 == str2
@@ -194,9 +228,10 @@ partial def Inline.beq [BEq i] : Lean.Doc.Inline i → Lean.Doc.Inline i → Boo
   | .other container1 content1, .other container2 content2 => container1 == container2 && arrayEq beq content1 content2
   | _, _ => false
 
-instance instBEqLeanInline [BEq i] : BEq (Lean.Doc.Inline i) := ⟨Inline.beq⟩
+public instance instBEqLeanInline [BEq i] : BEq (Lean.Doc.Inline i) where
+  beq := private Inline.beq
 
-@[instance] abbrev instBEqInline [BEq genre.Inline] : BEq (Inline genre) := instBEqLeanInline
+@[instance] public abbrev instBEqInline [BEq genre.Inline] : BEq (Inline genre) := instBEqLeanInline
 
 private partial def Inline.hashCode [Hashable i] : Lean.Doc.Inline i → UInt64
   | .text str => mixHash 11 <| hash str
@@ -211,13 +246,13 @@ private partial def Inline.hashCode [Hashable i] : Lean.Doc.Inline i → UInt64
   | .concat c => mixHash 43 <| hash (c.map hashCode)
   | .other container content => mixHash 47 <| mixHash (hash container) (hash <| content.map hashCode)
 
-instance instHashableLeanInline [Hashable i] : Hashable (Lean.Doc.Inline i) where
-  hash := Inline.hashCode
+public instance instHashableLeanInline [Hashable i] : Hashable (Lean.Doc.Inline i) where
+  hash := private Inline.hashCode
 
-@[instance] abbrev instHashableInline [Hashable genre.Inline] : Hashable (Inline genre) :=
+@[instance] public abbrev instHashableInline [Hashable genre.Inline] : Hashable (Inline genre) :=
   instHashableLeanInline
 
-@[instance] abbrev instOrdInline [Ord genre.Inline] : Ord (Inline genre) :=
+@[instance] public abbrev instOrdInline [Ord genre.Inline] : Ord (Inline genre) :=
   inferInstanceAs (Ord (Lean.Doc.Inline genre.Inline))
 
 private def reprArray (r : α → Nat → Format) (arr : Array α) : Format :=
@@ -233,7 +268,7 @@ private def reprCtor (c : Name) (args : List Format) : Format :=
   .nest 2 <| .group (.joinSep (.text s!"{c}" :: args) .line)
 
 -- The Lean instance exists, but shows the Lean constructor names instead of the Verso ones
-partial def Inline.reprPrec [Repr genre.Inline] (inline : Inline genre) (prec : Nat) : Std.Format :=
+public partial def Inline.reprPrec [Repr genre.Inline] (inline : Inline genre) (prec : Nat) : Std.Format :=
     open Repr Std.Format in
     let rec go i p :=
       (addAppParen · p) <|
@@ -257,93 +292,112 @@ partial def Inline.reprPrec [Repr genre.Inline] (inline : Inline genre) (prec : 
         | .other container content => reprCtor ``Inline.other [reprArg container, reprArray go content]
     go inline prec
 
-instance [Repr g.Inline] : Repr (Inline g) := ⟨Inline.reprPrec⟩
+public instance [Repr g.Inline] : Repr (Inline g) := ⟨Inline.reprPrec⟩
 
 
-def Inline.cast (inlines_eq : g1.Inline = g2.Inline) : Inline g1 → Inline g2 :=
+public def Inline.cast (inlines_eq : g1.Inline = g2.Inline) : Inline g1 → Inline g2 :=
   Lean.Doc.Inline.cast inlines_eq
 
 open Lean in
-inductive ArgVal where
+public inductive ArgVal where
   | name (x : Ident)
   | str (text : StrLit)
   | num (n : NumLit)
 deriving Repr, Inhabited, BEq
 
-def ArgVal.syntax (argVal : ArgVal) : Lean.Syntax :=
+public def ArgVal.syntax (argVal : ArgVal) : Lean.Syntax :=
   match argVal with
   | .name x => x
   | .str txt => txt
   | .num n => n
 
 open Lean in
-inductive Arg where
+public inductive Arg where
   | anon (value : ArgVal)
   | named (stx : Syntax) (name : Ident) (value : ArgVal)
   | flag (stx : Syntax) (name : Ident) (value : Bool)
 deriving Repr, Inhabited, BEq
 
 open Lean in
-def Arg.syntax : Arg → Syntax
+public def Arg.syntax : Arg → Syntax
   | .anon v => v.syntax
   | .named stx .. | .flag stx .. => stx
-
 
 export Lean.Doc (ListItem ListItem.mk)
 
 private def ListItem.toJson (blockToJson : ToJson α) : ListItem α → Json
   | ⟨xs⟩ => json% {"contents": $(xs.map blockToJson.toJson)}
 
-instance [inst : ToJson α] : ToJson (ListItem α) := ⟨ListItem.toJson inst⟩
+public instance [inst : ToJson α] : ToJson (ListItem α) where
+  toJson := private ListItem.toJson inst
 
-def ListItem.reprPrec [Repr α] : ListItem α → Nat → Std.Format := Repr.reprPrec
+private def ListItem.fromJson? [FromJson α] (json : Json) : Except String (ListItem α) := do
+  let v ← json.getObjVal? "contents"
+  .mk <$> FromJson.fromJson? v
+
+private def ListItem.reprPrec [Repr α] : ListItem α → Nat → Std.Format := Repr.reprPrec
+
+public instance [Repr α] : Repr (ListItem α) where
+  reprPrec := private ListItem.reprPrec
 
 export Lean.Doc (DescItem DescItem.mk)
+
+private def DescItem.reprPrec [Repr α] [Repr β] : DescItem α β → Nat → Std.Format := Repr.reprPrec
+
+public instance [Repr α] [Repr β] : Repr (DescItem α β) where
+  reprPrec := private DescItem.reprPrec
+
 
 private def DescItem.toJson (inlineToJson : ToJson α) (blockToJson : ToJson β) : DescItem α β → Json
   | ⟨term, desc⟩ => json% {"term": $(term.map inlineToJson.toJson), "contents": $(desc.map blockToJson.toJson)}
 
-instance [inst : ToJson α] : ToJson (ListItem α) := ⟨ListItem.toJson inst⟩
+private def DescItem.fromJson? [FromJson α] [FromJson β] (json : Json) : Except String (DescItem α β) := do
+  let term ← json.getObjVal? "term" >>= (·.getArr?)
+  let contents ← json.getObjVal? "contents" >>= (·.getArr?)
+  let term ← term.mapM FromJson.fromJson?
+  let contents ← contents.mapM FromJson.fromJson?
+  return ⟨term, contents⟩
 
-def DescItem.reprPrec [Repr α] [Repr β] : DescItem α β → Nat → Std.Format := Repr.reprPrec
+public instance [FromJson α] [FromJson β] : FromJson (DescItem α β) where
+  fromJson? := private DescItem.fromJson?
 
 @[inherit_doc Lean.Doc.Block]
-abbrev Block (genre : Genre) : Type :=
+public abbrev Block (genre : Genre) : Type :=
   Lean.Doc.Block genre.Inline genre.Block
 
-@[inherit_doc Lean.Doc.Block.para, match_pattern]
-def Block.para (contents : Array (Inline genre)) : Block genre :=
+@[inherit_doc Lean.Doc.Block.para, expose, match_pattern]
+public def Block.para (contents : Array (Inline genre)) : Block genre :=
   Lean.Doc.Block.para (contents : Array (Inline genre))
 
-@[inherit_doc Lean.Doc.Block.code, match_pattern]
-def Block.code (content : String) : Block genre :=
+@[inherit_doc Lean.Doc.Block.code, expose, match_pattern]
+public def Block.code (content : String) : Block genre :=
   Lean.Doc.Block.code (content : String)
 
-@[inherit_doc Lean.Doc.Block.ul, match_pattern]
-def Block.ul (items : Array (ListItem (Block genre))) : Block genre :=
+@[inherit_doc Lean.Doc.Block.ul, expose, match_pattern]
+public def Block.ul (items : Array (ListItem (Block genre))) : Block genre :=
   Lean.Doc.Block.ul (items : Array (ListItem (Block genre)))
 
-@[inherit_doc Lean.Doc.Block.ol, match_pattern]
-def Block.ol (start : Int) (items : Array (ListItem (Block genre))) : Block genre :=
+@[inherit_doc Lean.Doc.Block.ol, expose, match_pattern]
+public def Block.ol (start : Int) (items : Array (ListItem (Block genre))) : Block genre :=
   Lean.Doc.Block.ol (start : Int) (items : Array (ListItem (Block genre)))
 
-@[inherit_doc Lean.Doc.Block.dl, match_pattern]
-def Block.dl (items : Array (DescItem (Inline genre) (Block genre))) : Block genre :=
+@[inherit_doc Lean.Doc.Block.dl, expose, match_pattern]
+public def Block.dl (items : Array (DescItem (Inline genre) (Block genre))) : Block genre :=
   Lean.Doc.Block.dl (items : Array (DescItem (Inline genre) (Block genre)))
 
-@[inherit_doc Lean.Doc.Block.blockquote, match_pattern]
-def Block.blockquote (items : Array (Block genre)) : Block genre :=
+@[inherit_doc Lean.Doc.Block.blockquote, expose, match_pattern]
+public def Block.blockquote (items : Array (Block genre)) : Block genre :=
   Lean.Doc.Block.blockquote (items : Array (Block genre))
 
-@[inherit_doc Lean.Doc.Block.concat, match_pattern]
-def Block.concat (content : Array (Block genre)) : Block genre :=
+@[inherit_doc Lean.Doc.Block.concat, expose, match_pattern]
+public def Block.concat (content : Array (Block genre)) : Block genre :=
   Lean.Doc.Block.concat (content : Array (Block genre))
 
-@[inherit_doc Lean.Doc.Block.other, match_pattern]
-def Block.other (container : genre.Block) (content : Array (Block genre)) : Block genre :=
+@[inherit_doc Lean.Doc.Block.other, expose, match_pattern]
+public def Block.other (container : genre.Block) (content : Array (Block genre)) : Block genre :=
   Lean.Doc.Block.other (container : genre.Block) (content : Array (Block genre))
 
-instance : Append (Lean.Doc.Block i b) where
+public instance : Append (Lean.Doc.Block i b) where
   append
     | .concat #[], x => x
     | x, .concat #[] => x
@@ -352,10 +406,40 @@ instance : Append (Lean.Doc.Block i b) where
     | x, .concat xs => .concat (#[x] ++ xs)
     | x, y => .concat #[x, y]
 
-@[instance] abbrev instAppendBlock : Append (Block genre) :=
+@[instance] public abbrev instAppendBlock : Append (Block genre) :=
   inferInstanceAs (Append (Lean.Doc.Block genre.Inline genre.Block))
 
-def Block.empty : Block genre := .concat #[]
+public def Block.empty : Block genre := .concat #[]
+
+public partial def Block.rewriteOtherM [Monad m]
+    (onInline :
+      (Inline genre1 → m (Inline genre2)) →
+      genre1.Inline → Array (Inline genre1) → m (Inline genre2))
+    (onBlock :
+      (Inline genre1 → m (Inline genre2)) →
+      (Block genre1 → m (Block genre2)) →
+      genre1.Block → Array (Block genre1) → m (Block genre2)) :
+    Block genre1 → m (Block genre2)
+  | .code s => pure <| .code s
+  | .para content => .para <$> content.mapM (·.rewriteOtherM onInline)
+  | .blockquote content => .blockquote <$> content.mapM (·.rewriteOtherM onInline onBlock)
+  | .concat content => .concat <$> content.mapM (·.rewriteOtherM onInline onBlock)
+  | .ol n items => .ol n <$> items.mapM fun ⟨content⟩ => (⟨·⟩) <$> content.mapM (·.rewriteOtherM onInline onBlock)
+  | .ul items => .ul <$> items.mapM fun ⟨content⟩ => (⟨·⟩) <$> content.mapM (·.rewriteOtherM onInline onBlock)
+  | .dl items => .dl <$> items.mapM fun ⟨term, desc⟩ => (⟨·, ·⟩) <$> term.mapM (·.rewriteOtherM onInline) <*> desc.mapM (·.rewriteOtherM onInline onBlock)
+  | .other container content =>
+    onBlock (Inline.rewriteOtherM onInline) (Block.rewriteOtherM onInline onBlock) container content
+
+public partial def Block.rewriteOther
+    (onInline :
+      (Inline genre1 → Inline genre2) →
+      genre1.Inline → Array (Inline genre1) → Inline genre2)
+    (onBlock :
+      (Inline genre1 → Inline genre2) →
+      (Block genre1 → Block genre2) →
+      genre1.Block → Array (Block genre1) → Block genre2) :
+    Block genre1 → Block genre2 :=
+  Block.rewriteOtherM (m := Id) onInline onBlock
 
 private partial def Block.toJson [ToJson i] [ToJson b] : Lean.Doc.Block i b → Json
   | .para contents => json% {"para": $contents}
@@ -367,12 +451,49 @@ private partial def Block.toJson [ToJson i] [ToJson b] : Lean.Doc.Block i b → 
   | .concat content => json% {"concat": $(content.map toJson)}
   | .other container content => json% {"other": {"container": $container, "content": $(content.map toJson)}}
 
-instance instToJsonLeanBlock [ToJson i] [ToJson b] : ToJson (Lean.Doc.Block i b) := ⟨Block.toJson⟩
+public instance instToJsonLeanBlock [ToJson i] [ToJson b] : ToJson (Lean.Doc.Block i b) where
+  toJson := private Block.toJson
 
-@[instance] abbrev instToJsonBLock [ToJson genre.Inline] [ToJson genre.Block] : ToJson (Block genre) :=
+@[instance] public abbrev instToJsonBLock [ToJson genre.Inline] [ToJson genre.Block] : ToJson (Block genre) :=
   instToJsonLeanBlock
 
-partial def Block.beq [BEq i] [BEq b] : Lean.Doc.Block i b → Lean.Doc.Block i b → Bool
+private partial def Block.fromJson? [FromJson i] [FromJson b] (json : Json) : Except String (Lean.Doc.Block i b) := do
+  let vals ← json.getObj?
+  if let some v := vals["para"]? then
+    .para <$> FromJson.fromJson? v
+  else if let some v := vals["code"]? then
+    .code <$> FromJson.fromJson? v
+  else if let some v := vals["ul"]? then
+    let items ← v.getArr?
+    have : FromJson (Lean.Doc.Block i b) := ⟨Block.fromJson?⟩
+    .ul <$> items.mapM (ListItem.fromJson?)
+  else if let some v := vals["ol"]? then
+    let start ← v.getObjValAs? _ "start"
+    let items ← v.getObjVal? "items" >>= (·.getArr?)
+    have : FromJson (Lean.Doc.Block i b) := ⟨Block.fromJson?⟩
+    .ol start <$> items.mapM (ListItem.fromJson?)
+  else if let some v := vals["dl"]? then
+    have : FromJson (Lean.Doc.Block i b) := ⟨Block.fromJson?⟩
+    .dl <$> FromJson.fromJson? v
+  else if let some v := vals["blockquote"]? then
+    let v ← v.getArr?
+    .blockquote <$> v.mapM Block.fromJson?
+  else if let some v := vals["concat"]? then
+    let v ← v.getArr?
+    .concat <$> v.mapM Block.fromJson?
+  else if let some v := vals["other"]? then
+    let container ← v.getObjVal? "container"
+    let content ← v.getObjVal? "content" >>= (·.getArr?)
+    .other <$> FromJson.fromJson? container <*> content.mapM fromJson?
+  else throw s!"Expected an object containing a block constructor name as a key, but got {json.compress}"
+
+public instance instFromJsonLeanBlock [FromJson i] [FromJson b] : FromJson (Lean.Doc.Block i b) where
+  fromJson? := private Block.fromJson?
+
+@[instance] public abbrev instFromJsonBlock [FromJson genre.Inline] [FromJson genre.Block] : FromJson (Block genre) :=
+  instFromJsonLeanBlock
+
+private partial def Block.beq [BEq i] [BEq b] : Lean.Doc.Block i b → Lean.Doc.Block i b → Bool
   | .para c1, .para c2 => c1 == c2
   | .code c1, .code c2 => c1 == c2
   | .ul i1, .ul i2 => arrayEq (fun | ⟨c1⟩, ⟨c2⟩ => arrayEq beq c1 c2) i1 i2
@@ -384,12 +505,13 @@ partial def Block.beq [BEq i] [BEq b] : Lean.Doc.Block i b → Lean.Doc.Block i 
   | .other b1 c1, .other b2 c2 => b1 == b2 && arrayEq beq c1 c2
   | _, _ => false
 
-instance instBEqLeanBlock [BEq genre.Inline] [BEq genre.Block] : BEq (Block genre) := ⟨Block.beq⟩
+public instance instBEqLeanBlock [BEq genre.Inline] [BEq genre.Block] : BEq (Block genre) where
+  beq := private Block.beq
 
-@[instance] abbrev instBEqBlock [BEq genre.Inline] [BEq genre.Block] : BEq (Block genre) := instBEqLeanBlock
+@[instance] public abbrev instBEqBlock [BEq genre.Inline] [BEq genre.Block] : BEq (Block genre) := instBEqLeanBlock
 
 -- Upstream has an instance, but the constructor names are the Lean ones rather than the Verso ones
-partial def Block.reprPrec [Repr genre.Inline] [Repr genre.Block] (inline : Block genre) (prec : Nat) : Std.Format :=
+private partial def Block.reprPrec [Repr genre.Inline] [Repr genre.Block] (inline : Block genre) (prec : Nat) : Std.Format :=
     open Repr Std.Format in
     open Lean.Doc in
     let rec go i p :=
@@ -399,24 +521,57 @@ partial def Block.reprPrec [Repr genre.Inline] [Repr genre.Block] (inline : Bloc
         | .code content => reprCtor ``Block.code [reprArg content]
         | .ul items => reprCtor ``Block.ul [reprArray (@ListItem.reprPrec _ ⟨go⟩) items]
         | .ol start items => reprCtor ``Block.ol [reprArg start, reprArray (@ListItem.reprPrec _ ⟨go⟩) items]
-        | .dl items => reprCtor ``Block.dl [reprArray (@DescItem.reprPrec _ _ _ ⟨go⟩) items]
+        | .dl items => reprCtor ``Block.dl [reprArray (@DescItem.reprPrec _ _ ⟨Inline.reprPrec⟩ ⟨go⟩) items]
         | .blockquote items => reprCtor ``Block.blockquote [reprArray go items]
         | .concat content => reprCtor ``Block.concat [reprArray go content]
         | .other container content => reprCtor ``Block.other [reprArg container, reprArray go content]
     go inline prec
 
-instance [Repr g.Inline] [Repr g.Block] : Repr (Block g) where
-  reprPrec b p := Block.reprPrec b p
+public instance [Repr g.Inline] [Repr g.Block] : Repr (Block g) where
+  reprPrec b p := private Block.reprPrec b p
 
 
-def Block.cast (inlines_eq : g1.Inline = g2.Inline) (blocks_eq : g1.Block = g2.Block) : Block g1 → Block g2 :=
+public def Block.cast (inlines_eq : g1.Inline = g2.Inline) (blocks_eq : g1.Block = g2.Block) : Block g1 → Block g2 :=
   Lean.Doc.Block.cast inlines_eq blocks_eq
 
 @[inherit_doc Lean.Doc.Part]
-abbrev Part (genre : Genre) := Lean.Doc.Part genre.Inline genre.Block genre.PartMetadata
+public abbrev Part (genre : Genre) := Lean.Doc.Part genre.Inline genre.Block genre.PartMetadata
 
-@[match_pattern]
-def Part.mk
+private partial def Part.toJson [ToJson i] [ToJson b] [ToJson p] (p : Lean.Doc.Part i b p) := json% {
+    "title" : $(p.title),
+    "titleString" : $(p.titleString),
+    "metadata" : $(p.metadata),
+    "content": $(p.content),
+    "subParts": $(p.subParts.map Part.toJson)
+  }
+
+public instance instToJsonLeanPart [ToJson i] [ToJson b] [ToJson p] : ToJson (Lean.Doc.Part i b p) where
+  toJson := private Part.toJson
+
+@[instance] public abbrev instToJsonPart
+    [ToJson genre.Inline] [ToJson genre.Block] [ToJson genre.PartMetadata] :
+    ToJson (Part genre) :=
+  instToJsonLeanPart
+
+private partial def Part.fromJson? [FromJson i] [FromJson b] [FromJson p]
+    (json : Json) : Except String (Lean.Doc.Part i b p) := do
+  have : FromJson (Lean.Doc.Part i b p) := ⟨Part.fromJson?⟩
+  .mk <$> json.getObjValAs? _ "title"
+    <*> json.getObjValAs? _ "titleString"
+    <*> json.getObjValAs? _ "metadata"
+    <*> json.getObjValAs? _ "content"
+    <*> json.getObjValAs? _ "subParts"
+
+public instance instFromJsonLeanPart [FromJson i] [FromJson b] [FromJson p] : FromJson (Lean.Doc.Part i b p) where
+  fromJson? := private Part.fromJson?
+
+@[instance] public abbrev instFromJsonPart
+    [FromJson genre.Inline] [FromJson genre.Block] [FromJson genre.PartMetadata] :
+    FromJson (Part genre) :=
+  instFromJsonLeanPart
+
+@[expose, match_pattern]
+public def Part.mk
     (title : Array (Inline genre))
     (titleString : String)
     (metadata : Option genre.PartMetadata)
@@ -425,30 +580,29 @@ def Part.mk
   Lean.Doc.Part.mk title titleString metadata content subParts
 
 @[inherit_doc Lean.Doc.Part.title]
-abbrev Part.title : Part genre → Array (Inline genre) := Lean.Doc.Part.title
+public abbrev Part.title : Part genre → Array (Inline genre) := Lean.Doc.Part.title
 
 @[inherit_doc Lean.Doc.Part.titleString]
-abbrev Part.titleString : Part genre → String := Lean.Doc.Part.titleString
+public abbrev Part.titleString : Part genre → String := Lean.Doc.Part.titleString
 
 @[inherit_doc Lean.Doc.Part.metadata]
-abbrev Part.metadata : Part genre → Option genre.PartMetadata := Lean.Doc.Part.metadata
+public abbrev Part.metadata : Part genre → Option genre.PartMetadata := Lean.Doc.Part.metadata
 
 @[inherit_doc Lean.Doc.Part.content]
-abbrev Part.content : Part genre → Array (Block genre) := Lean.Doc.Part.content
+public abbrev Part.content : Part genre → Array (Block genre) := Lean.Doc.Part.content
 
 @[inherit_doc Lean.Doc.Part.subParts]
-abbrev Part.subParts : Part genre → Array (Part genre) := Lean.Doc.Part.subParts
-
+public abbrev Part.subParts : Part genre → Array (Part genre) := Lean.Doc.Part.subParts
 
 @[instance]
-abbrev instBEqPart [BEq genre.Inline] [BEq genre.Block] [BEq genre.PartMetadata] : BEq (Part genre) :=
+public abbrev instBEqPart [BEq genre.Inline] [BEq genre.Block] [BEq genre.PartMetadata] : BEq (Part genre) :=
   inferInstanceAs (BEq (Lean.Doc.Part genre.Inline genre.Block genre.PartMetadata))
 
-def Part.withoutSubparts (p : Part genre) : Part genre := { p with subParts := #[] }
+public def Part.withoutSubparts (p : Part genre) : Part genre := { p with subParts := #[] }
 
-def Part.withoutMetadata (p : Part genre) : Part genre := { p with metadata := none }
+public def Part.withoutMetadata (p : Part genre) : Part genre := { p with metadata := none }
 
-partial def Part.reprPrec [Repr genre.Inline] [Repr genre.Block] [Repr genre.PartMetadata] (part : Part genre) (_prec : Nat) : Std.Format :=
+private partial def Part.reprPrec [Repr genre.Inline] [Repr genre.Block] [Repr genre.PartMetadata] (part : Part genre) (_prec : Nat) : Std.Format :=
   open Std.Format in
   reprCtor ``Part.mk [
       reprArg (part.title : Array (Inline genre)),
@@ -458,15 +612,16 @@ partial def Part.reprPrec [Repr genre.Inline] [Repr genre.Block] [Repr genre.Par
       reprArray Part.reprPrec (part.subParts : Array (Part genre))
     ]
 
-instance [Repr g.Inline] [Repr g.Block] [Repr g.PartMetadata] : Repr (Part g) := ⟨Part.reprPrec⟩
+public instance [Repr g.Inline] [Repr g.Block] [Repr g.PartMetadata] : Repr (Part g) where
+  reprPrec := private Part.reprPrec
 
 /--
 Specifies how to modify the context while traversing the contents of a given part.
 -/
-class TraversePart (g : Genre) where
+public class TraversePart (g : Genre) where
   /--
   How to modify the context while traversing the contents of a given part. This is applied after
-  `part` and `genrePart` have rewritten the text, if applicable.
+  {lit}`part` and {lit}`genrePart` have rewritten the text, if applicable.
 
   It is also used during HTML generation.
   -/
@@ -475,7 +630,7 @@ class TraversePart (g : Genre) where
 /--
 Specifies how to modify the context while traversing the contents of a given block.
 -/
-class TraverseBlock (g : Genre) where
+public class TraverseBlock (g : Genre) where
   /--
   How to modify the context while traversing a given block.
 
@@ -484,9 +639,9 @@ class TraverseBlock (g : Genre) where
   inBlock : Block g → g.TraverseContext → g.TraverseContext := fun _ => id
 
 
-instance : TraversePart .none := {}
+public instance : TraversePart .none := {}
 
-instance : TraverseBlock .none := {}
+public instance : TraverseBlock .none := {}
 
 /--
 Genre-specific traversal.
@@ -495,93 +650,94 @@ The traversal pass is where cross-references are resolved. The traversal pass re
 genre-specific stateful computation until a fixed point is reached, both with respect to the state
 and the document. Traversal may update the state or rewrite parts of the document.
 
-The methods `part`, `block`, and `inline` provide effects to be carried out before traversing the
-given level of the AST, and `part` allows the part's metadata to be updated.
+{open Traverse}
+{open TraversePart}
 
-`genrePart` is carried out after `part`. It allows genre-specific rewriting of the entire part based
+The methods {name}`part`, {name}`block`, and {name full:=Verso.Doc.Traverse.inline}`inline` provide effects to be carried out before traversing the
+given level of the AST, and {name}`part` allows the part's metadata to be updated.
+
+{name}`genrePart` is carried out after {name}`part`. It allows genre-specific rewriting of the entire part based
 on genre-specific metadata. This is typically used to construct a table of contents or permalinks,
-but it can in principle arbitrarily rewrite the part. `inPart` is used to locally transform the
-genre's traversal context along the lines of `withReader`, and can be used to keep track of e.g. the
+but it can in principle arbitrarily rewrite the part. {name}`inPart` is used to locally transform the
+genre's traversal context along the lines of {name}`withReader`, and can be used to keep track of e.g. the
 current position in the table of contents.
 
-`genreBlock` and `genreInline` are invoked when traversal encounters `Block.other` and
-`Inline.other`. It may rewrite them, or have state effects.
+{name}`genreBlock` and {name}`genreInline` are invoked when traversal encounters {name}`Block.other` and
+{name}`Inline.other`. It may rewrite them, or have state effects.
 
 -/
-class Traverse (g : Genre) (m : outParam (Type → Type)) where
+public class Traverse (g : Genre) (m : outParam (Type → Type)) where
   /--
-  The effects carried out before traversing a `Part`.
+  The effects carried out before traversing a {name}`Part`.
   -/
   part [MonadReader g.TraverseContext m] [MonadState g.TraverseState m] : Part g → m (Option g.PartMetadata)
   /--
-  The effects carried out before traversing a `Block`.
+  The effects carried out before traversing a {name}`Block`.
   -/
   block [MonadReader g.TraverseContext m] [MonadState g.TraverseState m] : Block g → m Unit
   /--
-  The effects carried out before traversing an `Inline`.
+  The effects carried out before traversing an {name}`Inline`.
   -/
   inline [MonadReader g.TraverseContext m] [MonadState g.TraverseState m] : Inline g → m Unit
   /--
-  Operations carried out after `part`, when a part has metadata. It allows genre-specific rewriting
+  {open Traverse}
+
+  Operations carried out after {name}`part`, when a part has metadata. It allows genre-specific rewriting
   of the entire part based on genre-specific metadata. This is typically used to construct a table
   of contents or permalinks, but it can in principle arbitrarily rewrite the part. If it returns
-  `none`, then no rewrite is performed.
+  {name}`none`, then no rewrite is performed.
   -/
   genrePart [MonadReader g.TraverseContext m] [MonadState g.TraverseState m] : g.PartMetadata → Part g → m (Option (Part g))
   /--
-  The traversal of genre-specific block values. If it returns `none`, then no rewrite is performed.
+  The traversal of genre-specific block values. If it returns {name}`none`, then no rewrite is performed.
   -/
   genreBlock [MonadReader g.TraverseContext m] [MonadState g.TraverseState m] : g.Block → Array (Block g) → m (Option (Block g))
   /--
-  The traversal of genre-specific inline values. If it returns `none`, then no rewrite is performed.
+  The traversal of genre-specific inline values. If it returns {name}`none`, then no rewrite is performed.
   -/
   genreInline [MonadReader g.TraverseContext m] [MonadState g.TraverseState m] : g.Inline → Array (Inline g) → m (Option (Inline g))
 
+section
+variable (g : Genre) [Traverse g m] [TraversePart g] [TraverseBlock g] [Monad m]
+variable [MonadReader g.TraverseContext m] [MonadWithReader g.TraverseContext m]
+variable [MonadState g.TraverseState m]
 
 
-partial def Genre.traverse (g : Genre)
-    [Traverse g m] [TraversePart g] [TraverseBlock g] [Monad m]
-    [MonadReader g.TraverseContext m] [MonadWithReader g.TraverseContext m]
-    [MonadState g.TraverseState m]
-    (top : Part g) : m (Part g) :=
-  part top
+public partial def Genre.traverseInline (i : Doc.Inline g) : m (Doc.Inline g) := do
+  Traverse.inline i
+  match i with
+  | .emph content => .emph <$> content.mapM traverseInline
+  | .bold content => .bold <$> content.mapM traverseInline
+  | .link content ref => (.link · ref) <$> content.mapM traverseInline
+  | .footnote name content => .footnote name <$> content.mapM traverseInline
+  | .image alt ref => pure <| .image alt ref
+  | .concat content => .concat <$> content.mapM traverseInline
+  | .other container content => do
+    match ← Traverse.genreInline container content with
+    | .none => .other container <$> content.mapM traverseInline
+    | .some i' => traverseInline i'
+  | .text .. | .linebreak .. | .code .. | .math .. => pure i
 
-where
-  inline (i : Doc.Inline g) : m (Doc.Inline g) := do
-    Traverse.inline i
-    match i with
-    | .emph content => .emph <$> content.mapM inline
-    | .bold content => .bold <$> content.mapM inline
-    | .link content ref => (.link · ref) <$> content.mapM inline
-    | .footnote name content => .footnote name <$> content.mapM inline
-    | .image alt ref => pure <| .image alt ref
-    | .concat content => .concat <$> content.mapM inline
+public partial def Genre.traverseBlock (b : Doc.Block g) : m (Doc.Block g) := do
+  Traverse.block b
+  withReader (TraverseBlock.inBlock b) <|
+    match b with
+    | .para contents => .para <$> contents.mapM g.traverseInline
+    | .ul items => .ul <$> items.mapM fun
+      | ListItem.mk contents => ListItem.mk <$> contents.mapM traverseBlock
+    | .ol start items => .ol start <$> items.mapM fun
+      | ListItem.mk contents => ListItem.mk <$> contents.mapM traverseBlock
+    | .dl items => .dl <$> items.mapM fun
+      | DescItem.mk t d => DescItem.mk <$> t.mapM g.traverseInline <*> d.mapM traverseBlock
+    | .blockquote items => .blockquote <$> items.mapM traverseBlock
+    | .concat items => .concat <$> items.mapM traverseBlock
     | .other container content => do
-      match ← Traverse.genreInline container content with
-      | .none => .other container <$> content.mapM inline
-      | .some i' => inline i'
-    | .text .. | .linebreak .. | .code .. | .math .. => pure i
+      match ← Traverse.genreBlock container content with
+      | .none => .other container <$> content.mapM traverseBlock
+      | .some b' => traverseBlock b'
+    | .code .. => pure b
 
-  block (b : Doc.Block g) : m (Doc.Block g) := do
-    Traverse.block b
-    withReader (TraverseBlock.inBlock b) <|
-      match b with
-      | .para contents => .para <$> contents.mapM inline
-      | .ul items => .ul <$> items.mapM fun
-        | ListItem.mk contents => ListItem.mk <$> contents.mapM block
-      | .ol start items => .ol start <$> items.mapM fun
-        | ListItem.mk contents => ListItem.mk <$> contents.mapM block
-      | .dl items => .dl <$> items.mapM fun
-        | DescItem.mk t d => DescItem.mk <$> t.mapM inline <*> d.mapM block
-      | .blockquote items => .blockquote <$> items.mapM block
-      | .concat items => .concat <$> items.mapM block
-      | .other container content => do
-        match ← Traverse.genreBlock container content with
-        | .none => .other container <$> content.mapM block
-        | .some b' => block b'
-      | .code .. => pure b
-
-  part (p : Doc.Part g) : m (Doc.Part g) := do
+public partial def Genre.traversePart (p : Doc.Part g) : m (Doc.Part g) := do
     let meta' ← Traverse.part p
     let mut p := meta'.map ({ p with metadata := ·}) |>.getD p
     if let some md := p.metadata then
@@ -589,5 +745,8 @@ where
         p := p'
     let .mk title titleString metadata content subParts := p
     let (content', subParts') ← withReader (TraversePart.inPart p) <|
-      (·,·) <$> content.mapM block <*> subParts.mapM part
-    pure <| .mk (← title.mapM inline) titleString metadata content' subParts'
+      (·,·) <$> content.mapM g.traverseBlock <*> subParts.mapM traversePart
+    pure <| .mk (← title.mapM g.traverseInline) titleString metadata content' subParts'
+
+public partial def Genre.traverse (top : Part g) : m (Part g) :=
+  g.traversePart top
