src/verso/Verso/Hover.lean
@@ -3,36 +3,48 @@ Copyright (c) 2023-2024 Lean FRO LLC. All rights reserved.
 Released under Apache 2.0 license as described in the file LICENSE.
 Author: David Thrane Christiansen
 -/
+module
+public import Lean.Elab.InfoTree
+public import Lean.Message
 
-import Lean.Elab.InfoTree
-import Lean.Message
+set_option doc.verso true
 
 namespace Verso.Hover
 
 open Lean Elab
 
-inductive UserHover where
+/-!
+Lean's built-in hover mechanism isn't particularly extensible, so {module -checked}`Verso.Doc.Lsp`
+contains a number of custom handlers that use custom info tree entries to add Verso-related
+features.
+
+This module contains the underlying data representation used by these extensions, as well as
+user-facing API for adding custom hover annotations.
+-/
+
+public inductive UserHover where
   /-- A Markdown string to send as the hover -/
   | markdown (markedString : String)
   | messageData (messageData : MessageData)
 
-def CustomHover.toString (hover : UserHover) : IO String :=
+public def CustomHover.toString (hover : UserHover) : IO String :=
   match hover with
   | .markdown str => pure str
   | .messageData m => m.toString
 
-instance : Coe String UserHover where
+public instance : Coe String UserHover where
   coe := .markdown
 
-instance : Coe MessageData UserHover where
+public instance : Coe MessageData UserHover where
   coe := .messageData
 
-structure CustomHover where
+/-- A custom info node to save in the {name (full := Info.ofCustomInfo)}`ofCustomInfo` -/
+public structure CustomHover where
   /-- A Markdown string to send as the hover -/
   markedString : String
 deriving TypeName
 
-def addCustomHover [Monad m] [MonadInfoTree m] [MonadLiftT BaseIO m] (stx : Syntax) (hover : UserHover) : m Unit := do
+public def addCustomHover [Monad m] [MonadInfoTree m] [MonadLiftT BaseIO m] (stx : Syntax) (hover : UserHover) : m Unit := do
   let txt ← match hover with
     | .markdown str => pure str
     | .messageData m => m.toString
